extraction/theories/EAll.v
@@ -1,1 +1,1 @@
-From TemplateExtraction Require Export EAst EInduction ELiftSubst EUnivSubst ETyping EWcbvEval Extract.
+From TemplateExtraction Require Export EAst EInduction ELiftSubst ETyping EWcbvEval Extract.
