extraction/theories/EInduction.v
@@ -1,6 +1,6 @@
 (* Distributed under the terms of the MIT license.   *)
 
-From Template Require Import univ utils Ast AstUtils.
+From Template Require Import utils Ast AstUtils.
 From TemplateExtraction Require Import EAst.
 Require Import List Program.
 Require Import BinPos.
@@ -27,8 +27,8 @@ Lemma term_forall_list_ind :
     (forall (n : name) (t : term),
         P t -> forall t0 : term, P t0 -> P (tLetIn n t t0)) ->
     (forall t u : term, P t -> P u -> P (tApp t u)) ->
-    (forall (s : String.string) (u : list Level.t), P (tConst s u)) ->
-    (forall (i : inductive) (n : nat) (u : list Level.t), P (tConstruct i n u)) ->
+    (forall (s : String.string), P (tConst s)) ->
+    (forall (i : inductive) (n : nat), P (tConstruct i n)) ->
     (forall (p : inductive * nat) (t : term),
         P t -> forall l : list (nat * term),
             tCaseBrsProp P l -> P (tCase p t l)) ->
