extraction/theories/Extraction.v
@@ -16,11 +16,10 @@ Extraction Blacklist config uGraph univ Ast String List Nat UnivSubst
            LiftSubst Induction Typing Retyping Checker.
 Set Warnings "-extraction-opaque-accessed".
 
-From TemplateExtraction Require Import EAst EAstUtils EUnivSubst EInduction ELiftSubst ETyping Extract.
+From TemplateExtraction Require Import EAst EAstUtils EInduction ELiftSubst ETyping Extract.
 
 Extraction Library EAst.
 Extraction Library EAstUtils.
-Extraction Library EUnivSubst.
 Extraction Library EInduction.
 Extraction Library ELiftSubst.
 Extraction Library ETyping.
